\begin{frame}{Ví dụ}
    \begin{align}
        \dot{x}&=Ax\left(t\right)+Bu\left(t\right), \\
        A&=\left[\begin{array}{cc}
        0 & 1\\
        1 & 0
        \end{array}\right],\\
        B &=\left[\begin{array}{c}
        1\\
        0
        \end{array}\right],\\
        \left[\begin{array}{ccc}
        0 & 1 & 1\\
        1 & 0 & 0
        \end{array}\right]&\leadsto\left[\begin{array}{ccc}
        \delta_{1} & \delta_{1}+1 & \delta_{2}+1\\
        \delta_{1}+1 & \delta_{1} & \delta_{2}
        \end{array}\right].
    \end{align}
\end{frame}

\begin{frame}{Ví dụ}
    \begin{align}
        \left[A,B\right]&\leadsto\left[A,B\right]+D\Delta E, \\
        D&=\left[\begin{array}{c}
        1\\
        1
        \end{array}\right],\\
        E&=\left[\begin{array}{ccc}
        1 & 1 & 0\\
        0 & 0 & 1
        \end{array}\right].
    \end{align}
\end{frame}


\begin{frame}{Ví dụ}
    \begin{align}
        \left(E\left[A-\lambda I,B\right]^{-1}D\right)\left(v\right)
        &= E\left[A-\lambda I,B\right]^{-1}\left[\begin{array}{c}
1\\ 1\end{array}\right]v \nonumber\\
        &= E\left[A-\lambda I,B\right]^{-1}\left[\begin{array}{c}
v\\
v\end{array}\right]
    \end{align}
\end{frame}

\begin{frame}{Ví dụ}
    \begin{align}
        \left[A-\lambda I,B\right]^{-1}\left[\begin{array}{c}
        v\\
        v
        \end{array}\right]&=\left\{ \left[\begin{array}{c}
        p\\
        q\\
        r
        \end{array}\right]\colon\left[A-\lambda I,B\right]\left[\begin{array}{c}
        p\\
        q\\
        r
        \end{array}\right]=\left[\begin{array}{c}
        v\\
        v
        \end{array}\right],\,\forall p,q,r\in\C\right\} \nonumber\\
        %%% 
        &=\left\{ \left[\begin{array}{c}
        p\\
        q\\
        r
        \end{array}\right]\colon\left[\begin{array}{c}
        q+r-\lambda p\\
        q-p\lambda
        \end{array}\right]=\left[\begin{array}{c}
        v\\
        v
        \end{array}\right],\,\forall p,q,r\in\C\right\} .
    \end{align}
\end{frame}

\begin{frame}{Ví dụ}
    \begin{align}
        \left(E\left[A-\lambda I,B\right]^{-1}D\right)\left(v\right)&=\left\{ E\left[\begin{array}{c}
        p\\
        q\\
        r
        \end{array}\right]\colon\left[\begin{array}{c}
        q+r-\lambda p\\
        q-p\lambda
        \end{array}\right]=\left[\begin{array}{c}
        v\\
        v
        \end{array}\right],\,\forall p,q,r\in\C\right\} \nonumber\\
        %%
        &=\left\{ \left[\begin{array}{c}
        p+q\\
        r
        \end{array}\right]\colon\left[\begin{array}{c}
        q+r-\lambda p\\
        q-p\lambda
        \end{array}\right]=\left[\begin{array}{c}
        v\\
        v
        \end{array}\right],\,\forall p,q,r\in\C\right\} \nonumber\\
        %%
        &=\left\{ \left[\begin{array}{c}
        q+v+q\lambda\\
        v-q+\lambda\left(v+q\lambda\right)
        \end{array}\right]:q\in\C\right\} .
    \end{align}
\end{frame}

\begin{frame}{Ví dụ}
    \begin{align}
        ax_{1}+x_{2}&=b\\
        x_{1}&=q+v+q\lambda,\\
        x_{2}&=v-q+\lambda\left(v+q\lambda\right).
    \end{align}
    \begin{itemize}
        \item \(q = q_{0}\), \(q = q_{1}\) \(\implies\) \(a = 1 - \lambda\), \(b = 2v.\)
    \end{itemize}
    \begin{align}
        \left(1-\lambda\right)x_{1}+x_{2}&=2v,\\    
        x_{1}&=q+v+q\lambda,\\
        x_{2}&=v-q+\lambda\left(v+q\lambda\right).
    \end{align}
\end{frame}

\begin{frame}{Ví dụ}
\begin{itemize}
    \item \(\lambda = -1\)
        \begin{align}
            x_1 &= v,\\
            x_2 &= 0,\\
            d\left(0,\left(E\left[A-\lambda I,B\right]^{-1}D\right)\left(v\right)\right)&=\abs{v}.
        \end{align}
    \item \(\lambda\ne-1\),  \(\left(\C,\norm{\cdot}_{\infty}\right)\)
        \begin{align}
            2\abs v&=\abs{\left(1-\lambda\right)x_{1}+x_{2}} \nonumber\\
            &\le\abs{\left(1-\lambda\right)x_{1}}+\abs{x_{2}}\nonumber\\
            &\le\left(\left|1-\lambda\right|+1\right)\max\left\{ \left|x_{1}\right|,\left|x_{2}\right|\right\} \nonumber\\
            &=\left(\left|1-\lambda\right|+1\right)\norm{\left[\begin{array}{c}
                x_{1}\\
                x_{2}
            \end{array}\right]}_{\infty}
        \end{align}
    \end{itemize}
\end{frame}

\begin{frame}{Ví dụ}
\begin{itemize}
    \item \(\lambda\ne-1\),  \(\left(\C,\norm{\cdot}_{\infty}\right)\)
        \begin{align}
        \frac{2\left|v\right|}{\left|\lambda-1\right|+1}&\le\norm{\left[\begin{array}{c}
        x_{1}\\
        x_{2}
        \end{array}\right]}_{\infty}.
        \end{align}
    \item Dấu bằng:
    \begin{align}
        x_{1}&=e^{i\varphi}x_{2},\\
        x_{2}&=\frac{2v}{1+\left|\lambda-1\right|}\\
        -\left(\lambda-1\right)e^{i\varphi}&=\left|\lambda-1\right|
    \end{align}
    \end{itemize}
\end{frame}

\begin{frame}{Ví dụ}
    \begin{align}
        \norm{E\left[A-\lambda I,B\right]^{-1}D}&=\sup_{\left|v\right|=1}d\left(0,E\left[A-\lambda I,B\right]^{-1}D\left(v\right)\right) \nonumber\\
        %%
        &=\begin{cases}
        \sup_{\left|v\right|=1}\left\{ \inf\norm{\left[\begin{array}{c}
        x_{1}\\
        x_{2}
        \end{array}\right]}_{\infty}\right\}  & \lambda\ne-1,\\
        \sup_{\left|v\right|=1}\left\{ \inf\left|v\right|\right\}  & \lambda=-1,
        \end{cases} \nonumber\\
        %%
        &=\begin{cases}
        \sup_{\left|v\right|=1}\left\{ \frac{2\left|v\right|}{\left|\lambda-1\right|+1}\right\}  & \lambda\ne-1,\\
        \sup_{\left|v\right|=1}\left\{ \left|v\right|\right\}  & \lambda=-1,
        \end{cases} \nonumber\\
        %%
        &=\begin{cases}
        \frac{2}{\left|\lambda-1\right|+1}, & \lambda\ne-1,\\
        1 & \lambda=-1.
        \end{cases}
    \end{align}
\end{frame}


\begin{frame}{Ví dụ}
    \begin{align}
        \sup_{\lambda\in\C}\norm{E\left[A-\lambda I,B\right]^{-1}D}&=2,\\
        r_{\C}^{D,E}\left(A,B\right)&=\frac{1}{2}.
    \end{align}
\end{frame}



